Implement generic aligned_alloc

src/Main.fst
@@ -1113,6 +1113,47 @@ val slab_malloc (arena_id:US.t{US.v arena_id < US.v nb_arenas}) (bytes:U32.t)
 let slab_malloc arena_id bytes = (slab_malloc_i sc_list 0sz) arena_id bytes
 #pop-options
 
+
+/// `slab_aligned_alloc` works in a very similar way as `slab_malloc_i`
+/// The key difference lies in the condition of the if-branch: we only
+/// attempt to allocate in this size class if it satisfies the alignment
+/// constraint, i.e., alignment % size == 0
+[@@ reduce_attr]
+noextract
+let rec slab_aligned_alloc_i
+  (l:list sc{List.length l <= length sc_all.size_classes})
+  (i:US.t{US.v i + List.length l == US.v nb_size_classes})
+  (arena_id:US.t{US.v arena_id < US.v nb_arenas})
+  (alignment:U32.t)
+  bytes
+  : Steel (array U8.t)
+  emp
+  (fun r -> null_or_varray r)
+  (requires fun _ -> True)
+  (ensures fun _ r _ -> not (is_null r) ==> A.length r >= U32.v bytes)
+  = match l with
+    | [] -> return_null ()
+    | hd::tl ->
+      [@inline_let] let idx = (arena_id `US.mul` nb_size_classes) `US.add` i in
+      let size = index sc_all.ro_sizes idx in
+      if bytes `U32.lte` size && alignment `U32.rem` size = 0ul then
+        slab_malloc_one idx bytes
+      else
+        slab_aligned_alloc_i tl (i `US.add` 1sz) arena_id alignment bytes
+
+
+[@@ T.postprocess_with norm_full]
+val slab_aligned_alloc (arena_id:US.t{US.v arena_id < US.v nb_arenas}) (alignment:U32.t) (bytes:U32.t)
+  : Steel (array U8.t)
+  emp
+  (fun r -> null_or_varray r)
+  (requires fun _ -> True)
+  (ensures fun _ r _ -> not (is_null r) ==> A.length r >= U32.v bytes)
+
+#push-options "--fuel 0 --ifuel 0 --z3rlimit 100"
+let slab_aligned_alloc arena_id alignment bytes = (slab_aligned_alloc_i sc_list 0sz) arena_id alignment bytes
+#pop-options
+
 inline_for_extraction noextract
 let slab_free' (i:US.t{US.v i < US.v nb_size_classes * US.v nb_arenas}) (ptr: array U8.t) (diff: US.t)
   : Steel bool
